src/dafny/ssz/BoolSeDes.dfy
@@ -1,0 +1,30 @@
+
+include "../utils/NativeTypes.dfy"
+include "../utils/Eth2Types.dfy"
+
+/**
+ *  Boolean serialisation, desrialisation.
+ *
+ */
+ module BoolSeDes {
+
+    import opened NativeTypes
+    import opened Eth2Types
+
+    function method boolToBytes(b: bool) : seq<Byte> 
+        ensures | boolToBytes(b) | == 1 
+    {
+        if b then 
+            [1 as Byte]
+        else 
+            [0 as Byte]
+    }
+
+    function method bytesToBool(xs: seq<Byte>) : bool
+        requires | xs | == 1 
+    {
+       (xs[0] as nat) > 0
+    }
+
+
+ }
