src/dafny/ssz/IntSeDes.dfy
@@ -1,0 +1,45 @@
+
+include "../utils/NativeTypes.dfy"
+include "../utils/Eth2Types.dfy"
+
+/**
+ *  Integers serialisation, desrialisation.
+ *
+ */
+ module IntSeDes {
+
+    import opened NativeTypes
+    import opened Eth2Types
+
+    //  Uintk serialisation and deserielisation.
+
+    /** Uint8. */
+    function method uint8ToBytes(n: uint8) : seq<Byte> 
+        ensures |uint8ToBytes(n)| == 1
+    {
+        [n as Byte]
+    }
+ 
+
+    function method bytesToUint8(xs: seq<Byte>) : uint8
+        requires |xs| == 1
+    {
+        (xs[0] as uint8)
+        
+    }
+
+
+    /** Encode/decode Uint8 yields Identity. */
+    lemma uint8AsBytesInvolutive(n : uint8) 
+        ensures bytesToUint8(uint8ToBytes(n)) == n
+
+    /** Uint16. */
+    // function method bytesToUint16(xs: seq<Byte>) : uint16 
+    //     requires |xs| == 2
+
+    // function method uint16ToBytes(n : uint16) : seq<Byte> 
+    //     ensures |uint16ToBytes(n)| == 2
+    //     ensures bytesToUint16(uint16ToBytes(n)) == n
+
+   
+ }
